coq/theories/imperative/ImpSemantics.v
@@ -1,0 +1,319 @@
+Require Import impboot.utils.Core.
+Require Import impboot.utils.Llist.
+Require Import impboot.utils.Env.
+Require Import impboot.imperative.ImpSyntax.
+Require Import coqutil.Word.Interface.
+Require Import coqutil.Word.Naive.
+Require Import coqutil.Word.Properties.
+
+Inductive rresult {A : Type} {B : Type} : Type :=
+  | RRes (a : A)
+  | RRet (b : B)
+  | RErr
+  | RTimeOut.
+Arguments rresult : clear implicits.
+
+Notation "'dolet' v <- r1 ; r2" := (match r1 with
+  | RRes v => r2
+  | RRet v => RRet v
+  | RErr => RErr
+  | RTimeOut => RTimeOut
+  end) (at level 200, right associativity).
+
+Notation "'dolet' ( v1 , v2 ) <- r1 ; r2" := (match r1 with
+  | RRes (v1, v2) => r2
+  | RRet v => RRet v
+  | RErr => RErr
+  | RTimeOut => RTimeOut
+  end) (at level 200, right associativity).
+
+Notation "'dolet' ( v1 , v2 , v3 ) <- r1 ; r2" := (match r1 with
+  | RRes (v1, v2, v3) => r2
+  | RRet v => RRet v
+  | RErr => RErr
+  | RTimeOut => RTimeOut
+  end) (at level 200, right associativity).
+
+Notation "r1 ;; r2" := (dolet _ <- r1 ; r2)
+  (at level 200, right associativity).
+
+(* memory keys are in bytes *)
+Notation memory_t := (word64 -> option (option word64)) (only parsing).
+
+Record state := mkState {
+  funs : list ImpSyntax.func;
+  fuel : nat;
+  memory : memory_t;
+  alloc_addr : word64;
+  input : llist ascii;
+  output : list ascii
+}.
+
+Definition result A := rresult A (state * word64).
+
+Definition set_input (s : state) (inp : llist ascii) : state :=
+  {| funs := s.(funs);
+     fuel := s.(fuel);
+     memory := s.(memory);
+     alloc_addr := s.(alloc_addr);
+     input := inp;
+     output := s.(output) |}.
+
+Definition set_output (s : state) (out : list ascii) : state :=
+  {| funs := s.(funs);
+     fuel := s.(fuel);
+     memory := s.(memory);
+     alloc_addr := s.(alloc_addr);
+     input := s.(input);
+     output := out |}.
+
+Definition set_memory (s : state) (mem : memory_t) : state :=
+  {| funs := s.(funs);
+    fuel := s.(fuel);
+    memory := mem;
+    alloc_addr := s.(alloc_addr);
+    input := s.(input);
+    output := s.(output) |}.
+
+Definition set_fuel (s : state) (fuel : nat) : state :=
+  {| funs := s.(funs);
+    fuel := fuel;
+    memory := s.(memory);
+    alloc_addr := s.(alloc_addr);
+    input := s.(input);
+    output := s.(output) |}.
+
+Definition alloc_chunk (s : state) : result state :=
+  (* TODO(kπ) Check if there is no overflow in word64 (alloc_addr) *)
+  RRes {| funs := s.(funs);
+    fuel := s.(fuel);
+    memory := (fun a' => if word.eqb s.(alloc_addr) a' then Some None else s.(memory) a');
+    alloc_addr := word.add s.(alloc_addr) (word.of_Z 64);
+    input := s.(input);
+    output := s.(output) |}.
+
+Definition read_mem (a : word64) (s : state) : option word64 :=
+  match s.(memory) a with
+  | None => None
+  | Some opt => opt
+  end.
+
+Definition write_mem (a : word64) (w : word64) (s : state) : option state :=
+  match s.(memory) a with
+  | Some _ =>
+      Some (set_memory
+        s
+        (fun a' => if word.eqb a a' then Some (Some w) else s.(memory) a')
+      )
+  | _ => None
+  end.
+
+Definition init_state (inp : llist ascii) (fuel : nat) (funs : list ImpSyntax.func) : state :=
+  {| funs := funs;
+    memory := fun _ => None;
+    alloc_addr := word.of_Z 0;
+    fuel := fuel;
+    input := inp;
+    output := [] |}.
+
+Definition EOF_CONST : word64 := word.of_Z (0xFFFFFFFF : Z).
+
+Definition read_ascii (input : llist ascii) : (word64 * llist ascii) :=
+  match input with
+  | Lnil => (EOF_CONST, input)
+  | Lcons c cs => (word.of_Z (Z.of_nat (nat_of_ascii c)), cs)
+  end.
+
+Definition word_to_ascii (w : word64) : ascii :=
+  ascii_of_nat (Z.to_nat (word.unsigned w)).
+
+Fixpoint eval_exp (s : state) (env : IEnv.env) (e : exp) : result word64 :=
+  match e with
+  | Var n =>
+      match IEnv.lookup env n with
+      | Some v => RRes v
+      | None => RErr
+      end
+  | Const n => RRes n
+  | Add e1 e2 =>
+      dolet v1 <- eval_exp s env e1 ;
+      dolet v2 <- eval_exp s env e2 ;
+      RRes (word.add v1 v2)
+  | Sub e1 e2 =>
+      dolet v1 <- eval_exp s env e1 ;
+      dolet v2 <- eval_exp s env e2 ;
+      RRes (word.sub v1 v2)
+  | Div e1 e2 =>
+      dolet v1 <- eval_exp s env e1 ;
+      dolet v2 <- eval_exp s env e2 ;
+      if word.eqb v2 (word.of_Z 0)
+      then RErr
+      else RRes (word.divu v1 v2)
+  | Read a b =>
+      dolet va <- eval_exp s env a ;
+      dolet vb <- eval_exp s env b ;
+      (* convert index to byte offset *)
+      let addr := word.add va (word.mul vb (word.of_Z 64)) in
+      match read_mem addr s with
+      | Some v => RRes v
+      | _ => RErr
+      end
+  end.
+
+Fixpoint eval_exps (s : state) (env : IEnv.env) (es : list exp) : result (list word64) :=
+  match es with
+  | [] => RRes []
+  | e :: es =>
+    dolet v <- eval_exp s env e ;
+    dolet vs <- eval_exps s env es ;
+    RRes (v :: vs)
+  end.
+
+Fixpoint eval_test (s : state) (env : IEnv.env) (t : test) : result bool :=
+  match t with
+  | Test c e1 e2 =>
+      dolet v1 <- eval_exp s env e1 ;
+      dolet v2 <- eval_exp s env e2 ;
+      match c with
+      | Less => RRes (word.ltu v1 v2)
+      | Equal => RRes (word.eqb v1 v2)
+    end
+  | And t1 t2 =>
+    dolet v1 <- eval_test s env t1 ;
+    dolet v2 <- eval_test s env t2 ;
+    RRes (andb v1 v2)
+  | Or t1 t2 =>
+    dolet v1 <- eval_test s env t1 ;
+    dolet v2 <- eval_test s env t2 ;
+    RRes (orb v1 v2)
+  | Not t =>
+    dolet v <- eval_test s env t ;
+    RRes (negb v)
+  end.
+
+Definition find_func (fname : name) (s : state) :=
+  List.find (fun func => name_of_func func =? fname) s.(funs).
+
+(* size is in 64-byte chunks (size = 1 =:= 64 bytes) *)
+Definition allocate_memory (size : word64) (s : state) : result (word64 * state) :=
+  let number_of_chunks := Z.to_nat (word.unsigned size) in
+  let idxs := (List.seq 0 number_of_chunks) in
+  dolet s1 <- List.fold_left (fun acc_s _ =>
+    dolet acc_s_v <- acc_s ;
+    alloc_chunk acc_s_v
+  ) idxs (RRes s) ;
+  RRes (s.(alloc_addr), s1).
+
+Fixpoint make_env (names : list name) (values : list word64) (acc : IEnv.env) : IEnv.env :=
+  match names, values with
+  | [], [] => acc
+  | n :: names, v :: values =>
+    make_env names values (IEnv.insert (n, Some v) acc)
+  | _, _ => acc
+  end.
+
+(* TODO(kπ) Add fuel-based termination with the INTERP trick *)
+Fixpoint eval_cmd (s : state) (env : IEnv.env) (c : cmd)
+  (EVAL_CMD : forall (s:state)(env:IEnv.env)(c:cmd), result (IEnv.env*state))
+  (EVAL_CMDS : forall (s:state)(env:IEnv.env)(cs:list cmd), result (IEnv.env*state))
+  { struct c } : result (IEnv.env * state) :=
+  let eval_cmd s env c := eval_cmd s env c EVAL_CMD EVAL_CMDS in
+  let eval_cmds s env c := eval_cmds s env c EVAL_CMD EVAL_CMDS in
+  match c with
+  | Assign n e =>
+    dolet v <- eval_exp s env e ;
+    let env' := IEnv.insert (n, Some v) env in
+    RRes (env', s)
+  | Update a e e' =>
+    dolet va <- eval_exp s env a ;
+    dolet ve <- eval_exp s env e ;
+    dolet ve' <- eval_exp s env e' ;
+    match write_mem (word.add va ve) ve' s with
+    | Some s' => RRes (env, s')
+    | None => RErr
+    end
+  | If t c1 c2 =>
+    dolet cond <- eval_test s env t ;
+    if cond
+    then eval_cmds s env c1
+    else eval_cmds s env c2
+  | While t c =>
+    dolet cond <- eval_test s env t ;
+    if cond
+    then
+      dolet (env', s') <- eval_cmds s env c ;
+      EVAL_CMD s' env' (While t c)
+    else
+      RRes (env, s)
+  | Call n fname es =>
+    match find_func fname s with
+    | Some (Func _ params body) =>
+      if Nat.eqb (List.length params) (List.length es)
+      then
+        dolet args <- eval_exps s env es ;
+        let call_env := make_env params args IEnv.empty in
+        match EVAL_CMDS s call_env body with
+        | RRet (s', rw) => RRes (env, s')
+        | _ => RErr
+        end
+      else RErr
+    | None => RErr
+    end
+  | Return e =>
+  (* TODO(kπ) early return *)
+    dolet v <- eval_exp s env e ;
+    RRet (s, v)
+  (* TODO(kπ) Correct-ish up to here *)
+  | Alloc n e =>
+    dolet size <- eval_exp s env e ;
+    match allocate_memory size s with
+    | RRes (addr, s') =>
+      let env' := IEnv.insert (n, Some addr) env in
+      RRes (env', s')
+    | _ => RErr
+    end
+  | GetChar n =>
+    let (next_word, new_inp) := read_ascii s.(input) in
+    let env' := IEnv.insert (n, Some next_word) env in
+    RRes (env', set_input s new_inp)
+  | PutChar e =>
+    dolet v <- eval_exp s env e ;
+    let c := word_to_ascii v in
+    RRes (env, set_output s (s.(output) ++ [c]))
+  | Abort => RErr
+  end
+with eval_cmds (s : state) (env : IEnv.env) (cs : list cmd)
+  (EVAL_CMD : forall (s:state)(env:IEnv.env)(c:cmd), result (IEnv.env*state))
+  (EVAL_CMDS : forall (s:state)(env:IEnv.env)(cs:list cmd), result (IEnv.env*state))
+  { struct cs } : result (IEnv.env * state) :=
+  let eval_cmd s env c := eval_cmd s env c EVAL_CMD EVAL_CMDS in
+  let eval_cmds s env cs := eval_cmds s env cs EVAL_CMD EVAL_CMDS in
+  match cs with
+  | [] => RRes (env, s)
+  | c :: cs =>
+    dolet (env1, s1) <- EVAL_CMD s env c ;
+    eval_cmds s1 env1 cs
+  end.
+
+Fixpoint EVAL_CMD (fuel : nat) (s : state) (env : IEnv.env) (c : cmd)
+  { struct fuel } : result (IEnv.env * state) :=
+  match fuel with
+  | 0 => RTimeOut
+  | S fuel => eval_cmd s env c (EVAL_CMD fuel) (EVAL_CMDS fuel)
+  end
+with EVAL_CMDS (fuel : nat)  (s : state) (env : IEnv.env) (cs : list cmd)
+  { struct fuel } : result (IEnv.env * state) :=
+  match fuel with
+  | 0 => RTimeOut
+  | S fuel => eval_cmds s env cs (EVAL_CMD fuel) (EVAL_CMDS fuel)
+  end.
+
+Definition eval_prog (inp : llist ascii) (fuel : nat) (p : prog) : result state :=
+  match p with
+  | Program funcs =>
+    let call_main := Call 0 0 [] in
+    let s := init_state inp fuel funcs in
+    let env := IEnv.empty in
+    dolet (_, s') <- eval_cmd s env call_main (EVAL_CMD fuel) (EVAL_CMDS fuel) ;
+    RRes s'
+  end.
