coq/theories/utils/Env.v
@@ -1,0 +1,267 @@
+Require Import Coq.Logic.FunctionalExtensionality.
+From impboot Require Import utils.Core.
+
+Module Type EnvT.
+  Parameter env : Type.
+  Parameter empty : env.
+  Parameter name : Type.
+  Parameter Value : Type.
+  Parameter lookup : env -> name -> option Value.
+  Parameter insert : name * option Value -> env -> env.
+  Definition insert_some (p : name * Value) (v : env) : env :=
+    insert (fst p, Some (snd p)) v.
+  Parameter remove : name -> env -> env.
+
+  Axiom lookup_insert_eq : forall v x n,
+      lookup (insert (x, n) v) x = n.
+
+  Axiom lookup_insert_neq : forall v x1 x2 n,
+      x1 <> x2 ->
+      lookup (insert (x1, n) v) x2 = lookup v x2.
+
+  Axiom insert_insert_eq : forall v x n1 n2,
+      insert (x, n1) (insert (x, n2) v) = insert (x, n1) v.
+
+  Axiom insert_insert_neq : forall v x1 x2 n1 n2,
+      x1 <> x2 ->
+      insert (x1, n1) (insert (x2, n2) v) = insert (x2, n2) (insert (x1, n1) v).
+
+  Axiom insert_remove : forall v x n,
+      insert (x, n) (remove x v) = insert (x, n) v.
+
+  Axiom lookup_empty : forall x,
+      lookup empty x = None.
+
+  Axiom insert_lookup_self : forall n env,
+    insert (n, lookup env n) env = env.
+End EnvT.
+
+Require impboot.functional.FunSyntax.
+Require impboot.functional.FunValues.
+
+Module FEnv <: EnvT.
+  Definition name := FunSyntax.name.
+  Definition Value := FunValues.Value.
+  Definition eqb := Nat.eqb.
+  Definition env := name -> option Value.
+  Definition empty : env := fun _ => None.
+  Definition lookup (v : env) (x : name) : option Value := v x.
+  Definition insert (p : name * option Value) (v : env) : env :=
+    fun x => if Nat.eq_dec x (fst p) then (snd p) else v x.
+  Definition insert_some (p : name * Value) (v : env) : env :=
+    insert (fst p, Some (snd p)) v.
+  Definition remove (x : name) (v : env) : env :=
+    fun y => if Nat.eq_dec x y then None else v y.
+
+  Theorem lookup_insert_eq : forall v x n,
+      lookup (insert (x, n) v) x = n.
+  Proof.
+    intros; unfold lookup, insert, fst. destruct Nat.eq_dec; try reflexivity; congruence.
+  Qed.
+
+  Theorem lookup_insert_neq : forall v x1 x2 n,
+      x1 <> x2 ->
+      lookup (insert (x1, n) v) x2 = lookup v x2.
+  Proof.
+    intros; unfold lookup, insert, fst.
+    destruct Nat.eq_dec; try reflexivity.
+    congruence.
+  Qed.
+
+  Theorem insert_insert_eq : forall v x n1 n2,
+      insert (x, n1) (insert (x, n2) v) = insert (x, n1) v.
+  Proof.
+    intros; apply functional_extensionality; intros.
+    unfold insert; destruct Nat.eq_dec; reflexivity.
+  Qed.
+
+  Theorem insert_insert_neq : forall v x1 x2 n1 n2,
+      x1 <> x2 ->
+      insert (x1, n1) (insert (x2, n2) v) = insert (x2, n2) (insert (x1, n1) v).
+  Proof.
+    intros; apply functional_extensionality; intros.
+    unfold insert; destruct Nat.eq_dec eqn:?; try reflexivity.
+    unfold snd, fst in *.
+    destruct (Nat.eq_dec x x2) eqn:?; try reflexivity.
+    subst; congruence.
+  Qed.
+
+  Theorem insert_remove : forall v x n,
+      insert (x, n) (remove x v) = insert (x, n) v.
+  Proof.
+    intros; apply functional_extensionality; intros.
+    unfold insert, remove, fst; destruct Nat.eq_dec eqn:?; [reflexivity|].
+    destruct (Nat.eq_dec x x0) eqn:?; [|reflexivity].
+    subst; congruence.
+  Qed.
+
+  Theorem lookup_empty : forall x,
+      lookup empty x = None.
+  Proof. reflexivity. Qed.
+
+  Theorem insert_lookup_self : forall n env,
+    insert (n, lookup env n) env = env.
+  Proof.
+    intros; apply functional_extensionality; intros.
+    unfold insert, lookup, fst; destruct Nat.eq_dec eqn:?; [|reflexivity].
+    unfold snd; subst.
+    reflexivity.
+  Qed.
+End FEnv.
+
+Require impboot.imperative.ImpSyntax.
+Require Import coqutil.Word.Interface.
+Require Import coqutil.Word.Naive.
+Require Import coqutil.Word.Properties.
+
+Module IEnv <: EnvT.
+  Definition name := ImpSyntax.name.
+  Opaque name.
+  Definition Value := @word.rep 64 word64.
+  Opaque Value.
+  Definition env := name -> option Value.
+  Definition empty : env := fun _ => None.
+  Definition lookup (v : env) (x : name) : option Value := v x.
+  Definition insert (p : name * option Value) (v : env) : env :=
+    fun x => if Nat.eq_dec x (fst p) then (snd p) else v x.
+  Definition insert_some (p : name * Value) (v : env) : env :=
+    insert (fst p, Some (snd p)) v.
+  Definition remove (x : name) (v : env) : env :=
+    fun y => if Nat.eq_dec x y then None else v y.
+
+  Theorem lookup_insert_eq : forall v x n,
+      lookup (insert (x, n) v) x = n.
+  Proof.
+    intros; unfold lookup, insert, fst. destruct Nat.eq_dec; try reflexivity; congruence.
+  Qed.
+
+  Theorem lookup_insert_neq : forall v x1 x2 n,
+      x1 <> x2 ->
+      lookup (insert (x1, n) v) x2 = lookup v x2.
+  Proof.
+    intros; unfold lookup, insert, fst.
+    destruct Nat.eq_dec; try reflexivity.
+    congruence.
+  Qed.
+
+  Theorem insert_insert_eq : forall v x n1 n2,
+      insert (x, n1) (insert (x, n2) v) = insert (x, n1) v.
+  Proof.
+    intros; apply functional_extensionality; intros.
+    unfold insert; destruct Nat.eq_dec; reflexivity.
+  Qed.
+
+  Theorem insert_insert_neq : forall v x1 x2 n1 n2,
+      x1 <> x2 ->
+      insert (x1, n1) (insert (x2, n2) v) = insert (x2, n2) (insert (x1, n1) v).
+  Proof.
+    intros; apply functional_extensionality; intros.
+    unfold insert; destruct Nat.eq_dec eqn:?; try reflexivity.
+    unfold snd, fst in *.
+    destruct (Nat.eq_dec x x2) eqn:?; try reflexivity.
+    subst; congruence.
+  Qed.
+
+  Theorem insert_remove : forall v x n,
+      insert (x, n) (remove x v) = insert (x, n) v.
+  Proof.
+    intros; apply functional_extensionality; intros.
+    unfold insert, remove, fst; destruct Nat.eq_dec eqn:?; [reflexivity|].
+    destruct (Nat.eq_dec x x0) eqn:?; [|reflexivity].
+    subst; congruence.
+  Qed.
+
+  Theorem lookup_empty : forall x,
+      lookup empty x = None.
+  Proof. reflexivity. Qed.
+
+  Theorem insert_lookup_self : forall n env,
+    insert (n, lookup env n) env = env.
+  Proof.
+    intros; apply functional_extensionality; intros.
+    unfold insert, lookup, fst; destruct Nat.eq_dec eqn:?; [|reflexivity].
+    unfold snd; subst.
+    reflexivity.
+  Qed.
+End IEnv.
+
+(* Module MemEnv <: EnvT.
+  Definition name := @word.rep 64 word64.
+  Definition Value := @word.rep 64 word64.
+  Definition env := name -> option Value.
+  Definition empty : env := fun _ => None.
+  Definition lookup (v : env) (x : name) : option Value := v x.
+  Definition insert (p : name * option Value) (v : env) : env :=
+    fun x => if word.eqb x (fst p) then (snd p) else v x.
+  Definition insert_some (p : name * Value) (v : env) : env :=
+    insert (fst p, Some (snd p)) v.
+  Definition remove (x : name) (v : env) : env :=
+    fun y => if word.eqb x y then None else v y.
+
+  Theorem lookup_insert_eq : forall v x n,
+      lookup (insert (x, n) v) x = n.
+  Proof.
+    intros; unfold lookup, insert, fst.
+    rewrite word.unsigned_eqb.
+    destruct Z.eqb eqn:?; try reflexivity.
+    rewrite Z.eqb_refl in Heqb.
+    inversion Heqb.
+  Qed.
+
+  Theorem lookup_insert_neq : forall v x1 x2 n,
+      x1 <> x2 ->
+      lookup (insert (x1, n) v) x2 = lookup v x2.
+  Proof.
+    intros; unfold lookup, insert, fst.
+    destruct (word.eqb x2 x1) eqn:?; try reflexivity.
+    unfold snd.
+    apply word.eqb_true in Heqb.
+    congruence.
+  Qed.
+
+  Theorem insert_insert_eq : forall v x n1 n2,
+      insert (x, n1) (insert (x, n2) v) = insert (x, n1) v.
+  Proof.
+    intros; apply functional_extensionality; intros.
+    unfold insert, fst, snd.
+    destruct (word.eqb x0 x) eqn:?; try reflexivity.
+  Qed.
+
+  Theorem insert_insert_neq : forall v x1 x2 n1 n2,
+      x1 <> x2 ->
+      insert (x1, n1) (insert (x2, n2) v) = insert (x2, n2) (insert (x1, n1) v).
+  Proof.
+    intros; apply functional_extensionality; intros.
+    unfold insert, fst, snd; destruct (word.eqb x x1) eqn:?; try reflexivity.
+    destruct (word.eqb x x2) eqn:?; try reflexivity.
+    apply word.eqb_true in Heqb.
+    apply word.eqb_true in Heqb0.
+    subst; congruence.
+  Qed.
+
+  Theorem insert_remove : forall v x n,
+      insert (x, n) (remove x v) = insert (x, n) v.
+  Proof.
+    intros; apply functional_extensionality; intros.
+    unfold insert, remove, fst, snd.
+    destruct (word.eqb x0 x) eqn:?; try reflexivity.
+    destruct (word.eqb x x0) eqn:?; try reflexivity.
+    apply word.eqb_true in Heqb0.
+    apply word.eqb_false in Heqb.
+    subst; congruence.
+  Qed.
+
+  Theorem lookup_empty : forall x,
+      lookup empty x = None.
+  Proof. reflexivity. Qed.
+
+  Theorem insert_lookup_self : forall n env,
+    insert (n, lookup env n) env = env.
+  Proof.
+    intros; apply functional_extensionality; intros.
+    unfold insert, lookup, fst, snd.
+    destruct (word.eqb x n) eqn:?; try reflexivity.
+    apply word.eqb_true in Heqb.
+    subst; reflexivity.
+  Qed.
+End MemEnv. *)
