coq/theories/utils/Llist.v
@@ -1,10 +1,10 @@
 CoInductive llist {A : Type} : Type :=
-| lnil : llist
-| lcons : A -> llist -> llist.
+| Lnil : llist
+| Lcons : A -> llist -> llist.
 Arguments llist : clear implicits.
 
 Definition ltail {A : Type} (l : llist A) : llist A :=
   match l with
-  | lnil => lnil
-  | lcons _ tl => tl
+  | Lnil => Lnil
+  | Lcons _ tl => tl
   end.
